examples/sep/language.v
@@ -1,6 +1,8 @@
+Add LoadPath "../..".
 Require Import Arith.
 Require Import List.
 Require Import msl.eq_dec.
+Import Relations. 
 
 Definition table (A B : Type) := list (A*B).
 
@@ -31,32 +33,120 @@ Definition stack := table var adr.
 Definition heap := table adr adr.
 Definition state := (stack * heap)%type.
 
-Definition bind_option (A B: Type) (f: option A) (g: A -> option B) : option B :=
-  match f with None => None | Some x => g x end.
-
-Implicit Arguments bind_option [A B].
-
-Notation "'do1' X '<-' A ';' B" := (bind_option A (fun X => B))
-   (at level 200, X ident, A at level 100, B at level 200).
-
 Inductive command := 
+| Skip : command
 | Assign: var -> var -> command
 | Load : var -> var -> command
 | Store: var -> var -> command
 | Seq: command -> command -> command.
 
-Fixpoint exec (c: command) (s: state) := 
- match c , s with
- | Assign x y , (stk,hp) => 
-                           do1 v <- table_get stk y; 
-                           Some (table_set x v stk, hp)
- | Load x y , (stk, hp) => 
-                           do1 v <- table_get stk y;
-                           do1 v' <- table_get hp v;
-                           Some (table_set x v' stk, hp)
- | Store x y, (stk, hp) => 
-                           do1 v <- table_get stk y;
-                           do1 p <- table_get stk x;
-                           Some (stk, table_set p v hp)
- | Seq c1 c2, s => do1 s' <- exec c1 s; exec c2 s'
+Inductive step: relation (command * state) :=
+| stepAssign: 
+        forall x y v stk hp,
+        table_get stk y = Some v ->
+        step (Assign x y, (stk,hp)) (Skip, (table_set x v stk, hp))
+| stepLoad: 
+        forall x y v v' stk hp,
+         table_get stk y = Some v ->
+         table_get hp v = Some v' ->
+         step (Load x y, (stk,hp)) (Skip, (table_set x v' stk, hp))
+| stepStore: 
+         forall x y v p stk hp,
+          table_get stk y = Some v ->
+          table_get stk x = Some p ->
+          step (Store x y, (stk,hp)) (Skip, (stk, table_set p v hp))
+| stepSeq0:
+         forall c2 s,
+         step (Seq Skip c2, s) (c2, s)
+| stepSeq1:
+         forall c1 c1' c2 s s',
+         step (c1,s) (c1',s') ->
+         step (Seq c1 c2, s) (Seq c1' c2, s').
+
+Inductive step': relation (list command * state)  :=
+| step'Skip:
+         forall k s,
+         step' (Skip :: k, s) (k,s)
+| step'Assign: 
+        forall x y v stk hp k,
+        table_get stk y = Some v ->
+        step' (Assign x y :: k, (stk,hp)) (k, (table_set x v stk, hp))
+| step'Load: 
+        forall x y v v' stk hp k,
+         table_get stk y = Some v ->
+         table_get hp v = Some v' ->
+         step' (Load x y :: k, (stk,hp)) (k, (table_set x v' stk, hp))
+| step'Store: 
+         forall x y v p stk hp k,
+          table_get stk y = Some v ->
+          table_get stk x = Some p ->
+          step' (Store x y :: k, (stk,hp)) (k, (stk, table_set p v hp))
+| step'Seq:
+         forall c1 c2 k s cs', 
+         step' (c1 :: c2 ::k, s) cs' ->
+         step' (Seq c1 c2 :: k, s) cs'.
+
+Fixpoint stackit (k: list command) (c: command) : command :=
+ match k with
+ | nil => c
+ | c'::k' => stackit k' (Seq c c')
  end.
+
+Definition stackit' (k: list command) : command :=
+ match k with nil => Skip | c::k' => stackit k' c end.
+
+(* Eval compute in stackit' (Skip :: Assign 0 1 :: Assign 0 2 :: Assign 0 3 :: nil). *)
+
+Ltac inv H := inversion H; clear H; subst.
+
+Lemma stackit_step:
+  forall s s' k c c',
+   step (c,s) (c',s') -> step (stackit k c, s) (stackit k c', s').
+Proof.
+ induction k; simpl; intros.
+ auto.
+ apply IHk.
+ apply stepSeq1. auto.
+Qed.
+
+Lemma step'_equiv:
+  forall k s k' s',
+  clos_refl_trans _ step' (k,s) (k', s') -> 
+  clos_refl_trans _ step (stackit' k, s) (stackit' k', s').
+Proof.
+ intros.
+ remember (k,s) as ks.
+ remember (k',s') as ks'.
+ apply clos_rt1n_rt; apply clos_rt_rt1n in H.
+ revert k s Heqks k' s' Heqks'; induction H; intros; subst.
+ inv Heqks'.
+ apply rt1n_refl.
+ destruct y as [k1 s1].
+ rename IHclos_refl_trans_1n into IH.
+ specialize (IH _ _ (eq_refl _) _ _ (eq_refl _)).
+ destruct k; simpl.
+ simpl. inv H.
+ apply clos_rt_rt1n.
+ eapply rt_trans.
+ 2: apply clos_rt1n_rt; apply IH.
+ clear -H.
+ revert k k1 H.
+ induction c; intros; inv H.
+ destruct k1; simpl. apply rt_refl.
+ apply rt_step; apply stackit_step; constructor.
+ destruct k1; simpl. apply rt_step; econstructor; eauto.
+ eapply rt_trans; apply rt_step; apply stackit_step;
+    repeat econstructor; eauto.
+ destruct k1; simpl. apply rt_step; econstructor; eauto.
+ eapply rt_trans; apply rt_step; apply stackit_step;
+    repeat econstructor; eauto.
+ destruct k1; simpl. apply rt_step; econstructor; eauto.
+ eapply rt_trans; apply rt_step; apply stackit_step;
+    repeat econstructor; eauto.
+ apply IHc1 in H5.
+ eapply rt_trans; [ | apply H5].
+ replace (stackit k (Seq c1 c2)) with (stackit (c2::k) c1).
+ apply rt_refl.
+ clear. induction k; simpl; auto.
+Qed.
+
